\begin{align}
\dot{\td{F}}^{\mathrm p}_{11} &= \dot{\td{d}}_{0}\,{\left(\frac{\tilde{\sigma }_{\mathrm{eff}}}{\tilde{\sigma }_{f}}-1\right)}^m\,\left(\frac{3\,\tilde{M}_{11}^{\mathrm{el}}\,\lambda _{11}}{2\,J\,\tilde{\sigma }_{\mathrm{eff}}}+\frac{3\,\tilde{M}_{12}^{\mathrm{el}}\,\lambda _{21}}{2\,J\,\tilde{\sigma }_{\mathrm{eff}}}\right)\heavi\\ 
\dot{\td{F}}^{\mathrm p}_{21} &= \dot{\td{d}}_{0}\,{\left(\frac{\tilde{\sigma }_{\mathrm{eff}}}{\tilde{\sigma }_{f}}-1\right)}^m\,\left(\frac{3\,\tilde{M}_{21}^{\mathrm{el}}\,\lambda _{11}}{2\,J\,\tilde{\sigma }_{\mathrm{eff}}}+\frac{3\,\tilde{M}_{22}^{\mathrm{el}}\,\lambda _{21}}{2\,J\,\tilde{\sigma }_{\mathrm{eff}}}\right) \heavi\\ 
\dot{\td{F}}^{\mathrm p}_{12} &= \dot{\td{d}}_{0}\,{\left(\frac{\tilde{\sigma }_{\mathrm{eff}}}{\tilde{\sigma }_{f}}-1\right)}^m\,\left(\frac{3\,\tilde{M}_{11}^{\mathrm{el}}\,\lambda _{12}}{2\,J\,\tilde{\sigma }_{\mathrm{eff}}}+\frac{3\,\tilde{M}_{12}^{\mathrm{el}}\,\lambda _{22}}{2\,J\,\tilde{\sigma }_{\mathrm{eff}}}\right) \heavi\\ 
\dot{\td{F}}^{\mathrm p}_{22} &= \dot{\td{d}}_{0}\,{\left(\frac{\tilde{\sigma }_{\mathrm{eff}}}{\tilde{\sigma }_{f}}-1\right)}^m\,\left(\frac{3\,\tilde{M}_{21}^{\mathrm{el}}\,\lambda _{12}}{2\,J\,\tilde{\sigma }_{\mathrm{eff}}}+\frac{3\,\tilde{M}_{22}^{\mathrm{el}}\,\lambda _{22}}{2\,J\,\tilde{\sigma }_{\mathrm{eff}}}\right) \heavi\\ 
\dot{\td{F}}^{\mathrm p}_{33} &= \frac{3\,\tilde{M}_{33}^{\mathrm{el}}\,\dot{\td{d}}_{0}\,\lambda _{33}\,{\left(\frac{\tilde{\sigma }_{\mathrm{eff}}}{\tilde{\sigma }_{f}}-1\right)}^m}{2\,J\,\tilde{\sigma }_{\mathrm{eff}}} \heavi
\end{align}
