\begin{align}
\tilde{S}^{\mathrm el}_{11} &= J^{c}\,\left(2\,E_{11}^{\mathrm{el}}\,\tilde{\mu }_{\mathrm{si}}+\tilde{\lambda }_{\mathrm{si}}\,\left(E_{11}^{\mathrm{el}}+E_{22}^{\mathrm{el}}+E_{33}^{\mathrm{el}}\right)\right) \\ 
\tilde{S}^{\mathrm el}_{21} &= 2\,E_{21}^{\mathrm{el}}\,J^{c}\,\tilde{\mu }_{\mathrm{si}} \\ 
\tilde{S}^{\mathrm el}_{12} &= 2\,E_{12}^{\mathrm{el}}\,J^{c}\,\tilde{\mu }_{\mathrm{si}} \\ 
\tilde{S}^{\mathrm el}_{22} &= J^{c}\,\left(2\,E_{22}^{\mathrm{el}}\,\tilde{\mu }_{\mathrm{si}}+\tilde{\lambda }_{\mathrm{si}}\,\left(E_{11}^{\mathrm{el}}+E_{22}^{\mathrm{el}}+E_{33}^{\mathrm{el}}\right)\right) \\ 
\tilde{S}^{\mathrm el}_{33} &= J^{c}\,\left(2\,E_{33}^{\mathrm{el}}\,\tilde{\mu }_{\mathrm{si}}+\tilde{\lambda }_{\mathrm{si}}\,\left(E_{11}^{\mathrm{el}}+E_{22}^{\mathrm{el}}+E_{33}^{\mathrm{el}}\right)\right) 
\end{align}
