\documentclass[../main.tex]{subfiles}


% \newcommand*{\rttensor}[1]{\boldsymbol{\mathrm{\underline{\underline{#1}}}}}

\setlength\parindent{0cm}


\begin{document}



\section{Mathematical Formulation}
The geometry considered is a thin film of Silicon in the domain $ -L/2 \le X \le L/2$ and $0 \le Y \le H$. Consider a certain particle, initially located at the coordinate \textbf{X}. During deformation, this particle follows a path 


\begin{gather}
\x = \x(\X,t)
\end{gather}

\vspace{0.25cm}
Let $\u(\X, t)$ be the displacement of a material particle located at $\X$. Then
\begin{align}
    \u(\X, t) = \x(\X, t) - \X = [u(\X, t), v(\X, t), w(\X, t)]^{\T}
\end{align}

Let the total deformation gradient be denoted by $\F$.
\begin{align}
    \F &= \pdiff{\x}{\X} = \nablaX \u + \I \\
    \E &= \fc{1}{2}(\F^\T \F - \I)
\end{align}
Assuming plane strain deformation, 
\begin{align}
\F = 
\begin{bmatrix}
       1 + \pdiff{u}{X} && \pdiff{u}{Y} && 0 \\
       \pdiff{v}{X} && 1 + \pdiff{v}{\pd Y} && 0 \\
       0 && 0 && 1
\end{bmatrix} = \tensor{F}
\end{align}
Decomposition of deformation gradient gives, 
\begin{gather}
\F = \F^{\el} \F^{\inel}
\end{gather}
where $\F^{\el}$ and $\F^{\inel}$ are the deformation gradients due to elastic deformation and inelastic deformation respectively.

The inelastic deformation gradient tensor, $\F^{\inel}$, has contribution from two sources - deformation due to concentration gradient, $\F^\c$, and viscoplastic deformation, $\F^\p$.
\begin{align}
    \F^\inel = \F^\c \F^\p
\end{align}


\subsection{Viscoplastic Deformation}


\begin{align}
\dot{\F}^\p &= \inv{J} \fc{3}{2} \fc{\Mel \F^\p}{\sigmaeff} \dZEROdot \langle \fc{\sigmaeff}{\sigmaf} - 1 \rangle^\m  \\
\text{where, }\Mel &= J (\F^\el)^\T \DCS (\F^\el)^\mT \\
J &= \mathrm{det}(\F) 
\end{align}

$\F^{\rm{p}}$ is assumed to be of the following form:
\begin{align}
    \F^\p = \tensor{\lambda}
\end{align}

since, det($\F^\p$) = 1
\begin{gather}
     \lamzz = 1/(\lamxx \lamyy - \lamxy \lamyx)
\end{gather}



\subsection{Deformation due to concentration gradient}
\begin{align}
    \F^\c &= (\jc)^{1/3} \I \\
    \text{where } \jc &= 1 + 3 \eta \xmax \tc
\end{align}


\subsection{Momentum Conservation}

\begin{align}
    \F^\el &=  \F \inv{\F^\p \F^\c}
\end{align}






\begin{align}
\E^{\el} &= \fc{1}{2} \left[ (\F^\el)^\T \F^\el - \I \right]
\end{align}





Let $\PK$ and $\PKS$ denote the first and second Piola-Kirchhoff stress tensors respectively.

\begin{align}
    W(\F, c) &= \fc{\jc}{2}\fc{E(c)}{1 + \nu}\left( \fc{\nu}{1-2\nu}(\text{tr}\E^\el)^2 + \tr{\E^\el \E^\el}\right)
\end{align}

\begin{align}
    \PKS^\el &= \jc[2 \muSic \E^\el + \lamSic \tr{\E^\el}\I ]\\
    \PKS &= \inv{\F^\c} \inv{\F^\p} \PKS^\el \invT{\F^\p} \invT{\F^\c} \\
    \PK &= \F \PKS 
\end{align}




Let $\CS$ denote the Cauchy stress tensor. Then

\begin{align}
    \CS &= \inv{J} \PK \F^\T 
\end{align}




Let $\DCS$ denote the deviatoric part of the Cauchy stress, $\CS$; then

\begin{align}
    \DCS &= \CS - (1/3)\tr{\CS}\I \\
\end{align}


Let $\sigmaeff$ denote the von Mises stress. Then:

\begin{align}
    \sigmaeff = \sqrt{\fc{3}{2}{(\tau^2_{11} + \tau^2_{22} + \tau^2_{33}} + 2\tau^2_{12})}
\end{align}


\begin{gather}
\bm{\nabla}_\X \cdot \PK = 0.
\end{gather}

\subsection{Mass Convservation}
\begin{align}
    \pdiff{c}{t} &= - \bm{\nabla}_\X \cdot \bm{j}
\end{align}

\subsection{Non-Dimensionalization}
\begin{align*}
    \td{c} = c/c_\max && \td{\bm{j}} = \bm{j} H/(\cmax D_0) \\ \text{where, } \cmax = \chi_{\rm max}/V_m^B \\
    \tu = u/H && \tv = v/H \\
    \tX = X/H && \tY = Y/H \\
    \td{t} = D_0 t/H^2 && \tmusi, \tlamsi = \mu_{\text{si}}/E_0, \lambda_{\text{si}}/E_0 \\
    \td{E}(c) = E_{\text{si}}(1 + \eta_{\rm{E}} \chi_{\rm{max}} \td{c})/E_0 \text{, where }  E_0 = \fc{R_g T}{V_m^b} \\
    % \tsigma{0} = \fc{\sigma_0}{E_0}\\
    % \td{K} = \fc{K H}{E_0} \\
    % \td{G}_0 = \fc{G_0}{H E_0} \\
    % \td{\delta}_{\text{initiation}} = \fc{\delta_{\text{initiation}}}{H}\\
    % \td{\delta}_{\text{failure}} = \fc{\delta_{\text{failure}}}{H}
\end{align*}


\subsection{Definition of the state of charge}

\begin{align}
    \rm{soc} &= \fc{\int_{-L/2}^{L/2} \int_0^H \tc \rm{d}y \rm{d}x}{L H} \\
         &= H^2\fc{\int_{-L/2H}^{L/2H} \int_0^1 \tc(\td{x}, \td{y}) \rm{d}\td{y} \rm{d}\td{x}}{L H} \\
         &= H\fc{\int_{-L/2H}^{L/2H} \int_0^1 \tc(\td{x}, \td{y}) \rm{d}\td{y} \rm{d}\td{x}}{L} 
        %  &= 2 H\fc{\int_0^{L/2H} \int_0^1 \tc(\td{x}, \td{y}) \rm{d}\td{y} \rm{d}\td{x}}{L} \\
        %  &= \fc{2 H }{L} \rm{intop1}(\tc)
\end{align}

\subsection{Equations in component form}
\begin{align}
\F = 
\begin{bmatrix}
       1 + \pdiff{\tu}{\tX} && \pdiff{\tu}{\tY} && 0 \\
       \pdiff{\tv}{\tX} && 1 + \pdiff{\tv}{\tY} && 0 \\
       0 && 0 && 1
\end{bmatrix} = \begin{bmatrix}
    \tF{11} && \tF{12}  && 0 \\
    \tF{21} && \tF{22}  && 0 \\
    0 && 0 && \tF{33}
\end{bmatrix}
\end{align}

\input{./sections/equations/Fel_mat.tex}

\input{./sections/equations/Eel_mat.tex}

\input{./sections/equations/tSel_mat.tex}

\input{./sections/equations/tS_mat.tex}

\input{./sections/equations/tP_mat.tex}

\input{./sections/equations/tsigma_mat.tex}

\input{./sections/equations/ttau_mat.tex}


\begin{align}
    \tsigmaeff &= \sqrt{\fc{3}{2}(\ttau{11}^2 + \ttau{22}^2 + \ttau{33}^2 + 2\ttau{12}^2) }
\end{align}


\input{./sections/equations/tMel_mat.tex}

\textbf{Viscoplastic rates: }

\input{./sections/equations/Fpdot_mat.tex}


Viscoplastic rate equations in non-dimensional form:
\begin{align}
    \diff{\lamxx}{t} = \fc{1}{t_{\rm{ref}}}\diff{\lamxx}{\tt} = \fc{3\dot{d_0}}{2 J \tsigmaeff}(\tMel{11} \lamxx + \tMel{12}\lamyx)\HS(\fc{\tsigmaeff}{\tsigmaf} - 1 )^\m \\
   \diff{\lamxx}{\tt} = \fc{3\dot{\td{d}}_0}{2 J \tsigmaeff}(\tMel{11} \lamxx + \tMel{12}\lamyx)\HS(\fc{\tsigmaeff}{\tsigmaf} - 1 )^\m\\
   \text{where, } \dot{\td{d}}_0 = \dot{d_0} t_{\rm{ref}}
\end{align}

Stress equilibrium Equation:
\begin{align}
    \nablaX \cdot \PK &= \bm{0}.
\end{align}
\begin{align}
    \pdiff{P_{11}}{X} + \pdiff{P_{12}}{ Y} &= 0 \\
    \text{and, } \pdiff{P_{21}}{X} + \pdiff{P_{22}}{Y} &= 0
\end{align}
In non-dimensional form:
\begin{align}
    \fc{E_0}{H} \pdiff{\tP{11}}{\tX} + \fc{E_0}{H} \pdiff{\tP{12}}{\tY} &= 0 \\
    \text{and, } \fc{E_0}{H} \pdiff{\tP{21}}{\tX} + \fc{E_0}{H} \pdiff{\tP{22}}{\tY} &= 0 
\end{align}
So, 
\begin{align}
    \pdiff{\tP{11}}{\tX} + \pdiff{\tP{12}}{\tY} &= 0 \\
    \text{and, }   \pdiff{\tP{21}}{\tX} +  \pdiff{\tP{22}}{\tY} &= 0 
\end{align}
Mass conservation Equation:
\begin{align}
    \pdiff{c}{t} &= - \nablaX \cdot \bm{j} = -(\pdiff{j_x}{X} + \pdiff{j_y}{ Y}) \\
    \cmax \fc{D_0}{H^2} \pdiff{{\td{c}}}{\tt}  &= -(\fc{1}{H}\pdiff{ \td{j}_x}{\tX} + \fc{1}{H}\pdiff{ \td{j}_y}{\tY})\cmax \fc{D_0}{H} \\
    \text{so, }  \pdiff{{\tc}}{\tt}  &= - (\pdiff{ \td{j}_x}{\tX} +  \pdiff{ \td{j}_y}{\tY}) 
\end{align}


\textbf{For one way coupling:}
\begin{align}
 \bm{j} &= -D_0 \nablaX{c} \\
  \td{j}_x &= j_x H/(\cmax D_0)\\
                                &= -D_0 \pdiff{c}{X} H/(\cmax D_0)\\
                                &= -\pdiff{\tc}{\tX}\\
                    \td{j}_y &= j_y H/(\cmax D_0)\\
                    &= -\pdiff{\tc}{\tY}
\end{align}


\textbf{For two way coupling:}
\begin{align}
    \bm{j} &= - \fc{1}{R_g T} \fc{D\xmax \tc}{V^b_m} \inv{\F} \invT{\F} \nablaX \mu \\
    \bm{\td{j}} &= \frac{\bm{j} H}{\cmax D_0} =-\fc{1}{R_g T} \td{D} \tc \inv{\F} \invT{\F} \nablaX \mu \\
    D &= D_0 \rm{exp}(\fc{\alpha S_h}{E_0}) = D_0 \rm{exp}(\alpha \td{S}_h)= D_0 \rm{exp}\left(\alpha \frac{\td{S}_{11}+\td{S}_{33}}{2}\right) \\ 
    \mu &= \mu_0 + \mu_s; \td{\mu} = \frac{\mu}{R_g T} \\
    \mu_0 &= R_g T \text{log}(\gamma \td{c}); \td{\mu_0} = \text{log}(\gamma \td{c})\\
    \gamma &= \fc{1}{1-\td{c}}\text{exp}(\fc{1}{R_g T}[2(A_0 - 2B_0)\td{c} - 3(A_0 - B_0)(\td{c}^2)])\\
    \mu_s &= \fc{V_m^b}{\xmax}\left[-\fc{1}{3}\pdiff{\jc}{\tc}\tFel{im}\tFel{in}{C}_{mnkl}\tEel{kl} + \fc{1}{2}\left(\jc \pdiff{C_{ijkl}}{\tc} + \pdiff{\jc}{\tc} C_{ijkl}\right)\tEel{ij}\tEel{kl}\right] \\
    \td{\mu}_s &= \frac{1}{R_g T} \mu_s \\
        &= \fc{V_m^b}{R_g T \xmax}\left[-\fc{1}{3}\pdiff{\jc}{\tc}\tFel{im}\tFel{in}{C}_{mnkl}\tEel{kl} + \fc{1}{2}\left(\jc \pdiff{C_{ijkl}}{\tc} + \pdiff{\jc}{\tc} C_{ijkl}\right)\tEel{ij}\tEel{kl}\right] \\ 
        &= \fc{1}{\xmax}\left[-\fc{1}{3}\pdiff{\jc}{\tc}\tFel{im}\tFel{in}{\td{C}}_{mnkl}\tEel{kl} + \fc{1}{2}\left(\jc \pdiff{\td{C}_{ijkl}}{\tc} + \pdiff{\jc}{\tc} \td{C}_{ijkl}\right)\tEel{ij}\tEel{kl}\right] \\
    % \td{C}_{ijkl} &= \jc\left[\td{\lambda}_{si}(\tc)\delta_{ij} \delta_{kl} + \td{\mu}_{si}(\tc)(\delta_{ik} \delta_{jl} + \delta_{il} \delta_{jk})\right] \\
    \td{C}_{ijkl} \tEel{kl} &= \tPel{ij}  = \tSel{ij}/\jc \Longrightarrow \td{C}_{ijkl} = \td{\lambda}_{si}(\tc)\delta_{ij} \delta_{kl} +  \td{\mu}_{si}(\tc)(\delta_{ik} \delta_{jl} + \delta_{il} \delta_{jk})  \\
    \td{\mu}_s &= \fc{1}{\xmax}\left[-\fc{1}{3}\pdiff{\jc}{\tc}\tFel{im}\tFel{in}\tPel{mn} + \fc{1}{2}\jc \pdiff{\td{C}_{ijkl}}{\tc}\tEel{ij}\tEel{kl} + \fc{1}{2} \pdiff{\jc}{\tc} \td{C}_{ijkl}\tEel{ij}\tEel{kl}\right] \\
    &= \fc{1}{\xmax}\left[-\fc{1}{3}\pdiff{\jc}{\tc}\tFel{im}\tFel{in}\tPel{mn} + \fc{1}{2}\jc \pdiff{\td{C}_{ijkl}}{\tc}\tEel{ij}\tEel{kl} + \fc{1}{2} \pdiff{\jc}{\tc} \tEel{ij}\tPel{kl}\right] \\
    &= \fc{1}{\xmax}\left[\pdiff{\jc}{\tc} \tPel{mn} \left( -\fc{1}{3}\tFel{im}\tFel{in}+ \fc{1}{2} \tEel{mn}\right)+ \fc{1}{2}\jc \pdiff{\td{C}_{ijkl}}{\tc}\tEel{ij}\tEel{kl} \right] \\
    &= \fc{1}{\xmax}\left[\pdiff{\jc}{\tc} \tPel{mn} \left( -\fc{1}{3}(2\tEel{mn}+\delta_{mn})+ \fc{1}{2} \tEel{mn}\right)+ \fc{1}{2}\jc \pdiff{\td{C}_{ijkl}}{\tc}\tEel{ij}\tEel{kl} \right] \\
    &= \fc{1}{\xmax}\left[-\fc{1}{6}\pdiff{\jc}{\tc} \tPel{mn} \tEel{mn} - \fc{1}{3}\pdiff{\jc}{\tc} \tPel{mn}\delta_{mn} +  \fc{1}{2}\jc \pdiff{\td{C}_{ijkl}}{\tc}\tEel{ij}\tEel{kl} \right] \\
    &= \fc{1}{\xmax}\left[-\fc{1}{6}\pdiff{\jc}{\tc} \tPel{mn} \tEel{mn} - \fc{1}{3 }\pdiff{\jc}{\tc} \tPel{mm} +  \fc{1}{2}\jc \pdiff{\td{C}_{ijkl}}{\tc}\tEel{ij}\tEel{kl} \right] \\
    &= \frac{1}{\xmax}(\td{\mu}_1 + \td{\mu}_2 + \td{\mu}_3)
\end{align}



\begin{align}
    \td{\mu}_0 &= \text{log}(\gamma \td{c}) \\
    \td{\mu}_1 &= -\fc{1}{6}\pdiff{\jc}{\tc} [\tPel{11}\tEel{11} + \tPel{22}\tEel{22} + 2\tPel{12}\tEel{12} + \tPel{33}\tEel{33}] \\
    \td{\mu}_2 &= -\fc{1}{3}\pdiff{ \jc}{\tc}[\tPel{11} + \tPel{22} + \tPel{33}] \\
    \td{\mu}_3 &= \fc{1}{2}\jc \pdiff{ \td{C}_{ijkl}}{\tc}\tEel{kl}\tEel{ij} \\
    \pdiff{\td{C}_{ijkl}}{\tc} &= \pdiff{\td{\lambda}_{si}(\tc)}{\tc}\delta_{ij} \delta_{kl} +  \pdiff{\td{\mu}_{si}(\tc)}{\tc}(\delta_{ik} \delta_{jl} + \delta_{il} \delta_{jk})  \\
    \td{\mu}_3  &=  \fc{1}{2}\jc \pdiff{\td{\lambda}_{si}(\tc)}{\tc}\delta_{ij} \delta_{kl} \tEel{kl}\tEel{ij} + \fc{1}{2}\jc\pdiff{\td{\mu}_{si}(\tc)}{\tc}(\delta_{ik} \delta_{jl} \tEel{kl}\tEel{ij} + \delta_{il} \delta_{jk} \tEel{kl}\tEel{ij}) \\
    &=  \fc{1}{2}\jc \pdiff{\td{\lambda}_{si}(\tc)}{\tc} \tEel{kk}\tEel{ii} + \fc{1}{2}\jc\pdiff{\td{\mu}_{si}(\tc)}{\tc}(\tEel{ij}\tEel{ij} +  \tEel{ji}\tEel{ij}) \\
    &=  \fc{1}{2}\jc \pdiff{\td{\lambda}_{si}(\tc)}{\tc} (\mathrm{tr}(\mathbf{E^{\rm{el}}}))^2 + \jc\pdiff{\td{\mu}_{si}(\tc)}{\tc}\tEel{ij}\tEel{ij} \\
    &= \fc{1}{2}\jc[\tlamsi'(c)(\tEel{11} + \tEel{22} + \tEel{33})^2 + 2\tmusi'(\td{c})((\tEel{11})^2 + (\tEel{22})^2 + (\tEel{33})^2 + 2 (\tEel{12})^2)]\\
    \bm{j} &= - \fc{D\xmax \tc}{V^b_m} \td{\F}^{-1} (\td{\F}^{-1})^\T \nabla_{\X} \td \mu \\
    \bm{\td j} &= \bm{j}H V_m^b/(\chi_{\text{max}}D_0)\\
                &= -\fc{D}{D_0}H \tc \td{\F}^{-1}(\td{\F}^{-1})^\T \nabla_{\X} \td \mu\\
    \td{j}_x &= \fc{-\bar{D} H \tc}{J^2} \left(\pdiff{ \td \mu}{X}(\tF{12}^2 + \tF{22}^2) - \pdiff{ \td \mu}{ Y}(\tF{11}\tF{12} + \tF{21}\tF{22})\right)\\
    &= \fc{-\bar{D}  \tc}{J^2} \left(\pdiff{ \td \mu}{\tX}(\tF{12}^2 + \tF{22}^2) - \pdiff{ \td \mu}{\tY}(\tF{11}\tF{12} + \tF{21}\tF{22})\right)\\
    \td{j}_y &= \fc{-\bar{D} H \tc}{J^2} \left(\pdiff{ \td \mu}{Y}(\tF{11}^2 + \tF{21}^2) - \pdiff{ \td \mu}{X}(\tF{11}\tF{12} + \tF{21}\tF{22})\right)\\
    &= \fc{-\bar{D}  \tc}{J^2} \left( \pdiff{ \td \mu}{\tY}(\tF{11}^2 + \tF{21}^2) -\pdiff{ \td \mu}{\tX}(\tF{11}\tF{12} + \tF{21}\tF{22})\right)
\end{align}



\subsection{Boundary and Initial Conditions}
\begin{center}
    \begin{align}
        \tc(\tX, \tY, 0) = 0 \\
        \tu(\tX, \tY, 0) = 0 \\
        \tv(\tX, \tY, 0) = 0 \\
        \tu(\tX, 0, \tt) = \tv(\tX, 0, \tt) = 0 \\
        \tu(-1/2, \tY, \tt) =  \tu(1/2, \tY, \tt) = 0 \\
        \td{j}_x(\tX, 1, \tt) = \td{j}_0 (1 - \tc(\tX, 1, \tt))
     \end{align}     
\end{center}



\end{document}
