\begin{align}
F^{\mathrm el}_{11} &= \frac{F_{11}\,\lambda _{22}-F_{12}\,\lambda _{21}}{{J^{c}}^{1/3}\,\left(\lambda _{11}\,\lambda _{22}-\lambda _{12}\,\lambda _{21}\right)} \\ 
F^{\mathrm el}_{21} &= \frac{F_{21}\,\lambda _{22}-F_{22}\,\lambda _{21}}{{J^{c}}^{1/3}\,\left(\lambda _{11}\,\lambda _{22}-\lambda _{12}\,\lambda _{21}\right)} \\ 
F^{\mathrm el}_{12} &= -\frac{F_{11}\,\lambda _{12}-F_{12}\,\lambda _{11}}{{J^{c}}^{1/3}\,\left(\lambda _{11}\,\lambda _{22}-\lambda _{12}\,\lambda _{21}\right)} \\ 
F^{\mathrm el}_{22} &= -\frac{F_{21}\,\lambda _{12}-F_{22}\,\lambda _{11}}{{J^{c}}^{1/3}\,\left(\lambda _{11}\,\lambda _{22}-\lambda _{12}\,\lambda _{21}\right)} \\ 
F^{\mathrm el}_{33} &= \frac{1}{{J^{c}}^{1/3}\,\lambda _{33}} 
\end{align}
