\begin{align}
\dot{F}^{\mathrm p}_{11} &= \dot{d}_{0}\,{\left(\frac{\tilde{\sigma }_{\mathrm{eff}}}{\tilde{\sigma }_{f}}-1\right)}^m\,\left(\frac{3\,\tilde{M}_{11}^{\mathrm{el}}\,\lambda _{11}}{2\,J\,\tilde{\sigma }_{\mathrm{eff}}}+\frac{3\,\tilde{M}_{12}^{\mathrm{el}}\,\lambda _{21}}{2\,J\,\tilde{\sigma }_{\mathrm{eff}}}\right) \\ 
\dot{F}^{\mathrm p}_{21} &= \dot{d}_{0}\,{\left(\frac{\tilde{\sigma }_{\mathrm{eff}}}{\tilde{\sigma }_{f}}-1\right)}^m\,\left(\frac{3\,\tilde{M}_{21}^{\mathrm{el}}\,\lambda _{11}}{2\,J\,\tilde{\sigma }_{\mathrm{eff}}}+\frac{3\,\tilde{M}_{22}^{\mathrm{el}}\,\lambda _{21}}{2\,J\,\tilde{\sigma }_{\mathrm{eff}}}\right) \\ 
\dot{F}^{\mathrm p}_{12} &= \dot{d}_{0}\,{\left(\frac{\tilde{\sigma }_{\mathrm{eff}}}{\tilde{\sigma }_{f}}-1\right)}^m\,\left(\frac{3\,\tilde{M}_{11}^{\mathrm{el}}\,\lambda _{12}}{2\,J\,\tilde{\sigma }_{\mathrm{eff}}}+\frac{3\,\tilde{M}_{12}^{\mathrm{el}}\,\lambda _{22}}{2\,J\,\tilde{\sigma }_{\mathrm{eff}}}\right) \\ 
\dot{F}^{\mathrm p}_{22} &= \dot{d}_{0}\,{\left(\frac{\tilde{\sigma }_{\mathrm{eff}}}{\tilde{\sigma }_{f}}-1\right)}^m\,\left(\frac{3\,\tilde{M}_{21}^{\mathrm{el}}\,\lambda _{12}}{2\,J\,\tilde{\sigma }_{\mathrm{eff}}}+\frac{3\,\tilde{M}_{22}^{\mathrm{el}}\,\lambda _{22}}{2\,J\,\tilde{\sigma }_{\mathrm{eff}}}\right) \\ 
\dot{F}^{\mathrm p}_{33} &= \frac{3\,\tilde{M}_{33}^{\mathrm{el}}\,\dot{d}_{0}\,\lambda _{33}\,{\left(\frac{\tilde{\sigma }_{\mathrm{eff}}}{\tilde{\sigma }_{f}}-1\right)}^m}{2\,J\,\tilde{\sigma }_{\mathrm{eff}}} 
\end{align}
