\begin{align}
S_{11} &= \frac{S_{11}^{\mathrm{el}}\,{\lambda _{22}}^2+S_{22}^{\mathrm{el}}\,{\lambda _{12}}^2-S_{12}^{\mathrm{el}}\,\lambda _{12}\,\lambda _{22}-S_{21}^{\mathrm{el}}\,\lambda _{12}\,\lambda _{22}}{{J^{c}}^{2/3}\,{\left(\lambda _{11}\,\lambda _{22}-\lambda _{12}\,\lambda _{21}\right)}^2} \\ 
S_{21} &= \frac{S_{12}^{\mathrm{el}}\,\lambda _{12}\,\lambda _{21}-S_{22}^{\mathrm{el}}\,\lambda _{11}\,\lambda _{12}-S_{11}^{\mathrm{el}}\,\lambda _{21}\,\lambda _{22}+S_{21}^{\mathrm{el}}\,\lambda _{11}\,\lambda _{22}}{{J^{c}}^{2/3}\,{\left(\lambda _{11}\,\lambda _{22}-\lambda _{12}\,\lambda _{21}\right)}^2} \\ 
S_{12} &= \frac{S_{12}^{\mathrm{el}}\,\lambda _{11}\,\lambda _{22}-S_{22}^{\mathrm{el}}\,\lambda _{11}\,\lambda _{12}-S_{11}^{\mathrm{el}}\,\lambda _{21}\,\lambda _{22}+S_{21}^{\mathrm{el}}\,\lambda _{12}\,\lambda _{21}}{{J^{c}}^{2/3}\,{\left(\lambda _{11}\,\lambda _{22}-\lambda _{12}\,\lambda _{21}\right)}^2} \\ 
S_{22} &= \frac{S_{11}^{\mathrm{el}}\,{\lambda _{21}}^2+S_{22}^{\mathrm{el}}\,{\lambda _{11}}^2-S_{12}^{\mathrm{el}}\,\lambda _{11}\,\lambda _{21}-S_{21}^{\mathrm{el}}\,\lambda _{11}\,\lambda _{21}}{{J^{c}}^{2/3}\,{\left(\lambda _{11}\,\lambda _{22}-\lambda _{12}\,\lambda _{21}\right)}^2} \\ 
S_{33} &= \frac{S_{33}^{\mathrm{el}}}{{J^{c}}^{2/3}\,{\lambda _{33}}^2} 
\end{align}
